

Derivation of Gradient Descent

Cost function Linear regression \rightarrow MSE

$$J(w, b) = \frac{1}{2m} \sum_{i=1}^m (f_{w,b}(x^{(i)}) - y^{(i)})^2$$

where $f_{w,b}(x) = wx + b$ $m \rightarrow$ no. of samples

Gradient Descent algorithm \rightarrow

$$w = w - \alpha \frac{\partial J}{\partial w}(w, b)$$

$$b = b - \alpha \frac{\partial J}{\partial b}(w, b)$$

(Repeat till convergence)

$$\frac{\partial J}{\partial w}(w, b) = \frac{\partial}{\partial w} \frac{1}{2m} \sum_{i=1}^m (f_{w,b}(x^{(i)}) - y^{(i)})^2$$

$$\rightarrow \frac{1}{2m} \sum_{i=1}^m (wx^{(i)} + b - y^{(i)})^2 \cdot x^{(i)}$$

$$\rightarrow \frac{1}{m} \sum_{i=1}^m (wx^{(i)} + b - y^{(i)}) \cdot x^{(i)}$$

(By applying chain rule)

$$\frac{\partial J(w, b)}{\partial w} = \frac{1}{m} \sum_{i=1}^m (f_{w, b}(x^{(i)}) - y^{(i)}) \cdot x^{(i)}$$

$$\frac{\partial J(w, b)}{\partial b} = \frac{1}{2m} \sum_{i=1}^m (f_{w, b}(x^{(i)}) - y^{(i)})^2$$

$$\rightarrow \frac{1}{2m} \sum_{i=1}^m (wx^{(i)} + b - y^{(i)}) \cdot 2$$

$$= \frac{1}{m} \sum_{i=1}^m (wx^{(i)} + b - y^{(i)})$$

$$\frac{\partial J(w, b)}{\partial b} = \frac{1}{m} \sum_{i=1}^m (f_{w, b}(x^{(i)}) - y^{(i)})$$

$$w = w - \alpha \sum_{i=1}^m (f_{w, b}(x^{(i)}) - y^{(i)}) x^{(i)}$$

$$b = b - \alpha \sum_{i=1}^m (f_{w, b}(x^{(i)}) - y^{(i)})$$

Gradient Descent for linear
regression (ML(E))